coq/Translation/ForeignToJavaScriptAst.v
@@ -1,6 +1,4 @@
 (*
- * Copyright 2015-2016 IBM Corporation
- *
  * Licensed under the Apache License, Version 2.0 (the "License");
  * you may not use this file except in compliance with the License.
  * You may obtain a copy of the License at
@@ -14,7 +12,24 @@
  * limitations under the License.
  *)
 
-Require Export CommonRuntime.
-Require Export JavaScriptAst.
-Require Export JavaScriptAstUtil.
+Require Import List.
+Require Import String.
+Require Import Utils.
+Require Import ForeignRuntime.
+Require Import JavaScriptAstRuntime.
+
+Local Open Scope string_scope.
+
+Section ForeigntoJavaScriptAst.
+
+Class foreign_to_ajavascript {fruntime:foreign_runtime}: Type
+  := mk_foreign_to_ajavascript {
+         foreign_to_ajavascript_unary_op
+           (fu:foreign_unary_op_type)
+           (e:expr) : expr
+         ; foreign_to_ajavascript_binary_op
+             (fb:foreign_binary_op_type)
+             (e1 e2:expr) : expr
+       }.
+End ForeigntoJavaScriptAst.
 
