coq/Compiler/Driver/CompDriver.v
@@ -101,6 +101,7 @@ Section CompDriver.
   Require Import ForeignToCloudant.
   Require Import ForeignToJava.
   Require Import ForeignToJavaScript.
+  Require Import ForeignToJavaScriptAst.
   Require Import ForeignToScala.
 
   (** Compiler Driver *)
@@ -124,6 +125,7 @@ Section CompDriver.
   Context {nnrc_logger:optimizer_logger string nnrc}.
   Context {dnnrc_logger:optimizer_logger string (DNNRCBase.dnnrc_base fr (type_annotation unit) dataframe)}.
   Context {ftojs:foreign_to_javascript}.
+  Context {ftoajs:foreign_to_ajavascript}.
   Context {ftojava:foreign_to_java}.
   Context {ftos:foreign_to_scala}.
   Context {ftospark:foreign_to_spark}.
