coq/JavaScriptAst/Lang/JavaScriptAstUtil.v
@@ -1,0 +1,63 @@
+(*
+ * Copyright 2015-2016 IBM Corporation
+ *
+ * Licensed under the Apache License, Version 2.0 (the "License");
+ * you may not use this file except in compliance with the License.
+ * You may obtain a copy of the License at
+ *
+ * http://www.apache.org/licenses/LICENSE-2.0
+ *
+ * Unless required by applicable law or agreed to in writing, software
+ * distributed under the License is distributed on an "AS IS" BASIS,
+ * WITHOUT WARRANTIES OR CONDITIONS OF ANY KIND, either express or implied.
+ * See the License for the specific language governing permissions and
+ * limitations under the License.
+ *)
+
+Require Import List.
+Require Import CommonRuntime.
+Require Import JsAst.JsSyntax.
+Require Import JavaScriptAst.
+
+Section JavaScriptAstUtil.
+  Import ListNotations.
+
+  Definition empty_array := expr_array nil.
+
+  Definition array_push e1 e2 :=
+    (* use [array_proto_push_function_object] ? *)
+    expr_call (expr_member e1 "push") [ e2 ].
+
+  Definition array_get e1 e2 :=
+    expr_access e1 e2.
+
+  (** Runtime  functions *)
+
+  Definition brands_to_js_ast sl : expr :=
+    expr_array
+      (List.map
+         (fun s => Some (expr_literal (literal_string s)))
+         sl).
+
+  Definition sortCriteria_to_js_ast (sc: string * SortDesc) :=
+    let (lbl, c) := sc in
+    match c with
+    | Ascending =>
+      expr_object
+        [ (propname_identifier "asc", propbody_val (expr_literal (literal_string lbl))) ]
+    | Descending =>
+      expr_object
+        [ (propname_identifier "desc", propbody_val (expr_literal (literal_string lbl))) ]
+    end.
+
+  Definition sortCriterias_to_js_ast (scl: SortCriterias) :=
+    expr_array
+      (List.map
+         (fun sc => Some (sortCriteria_to_js_ast sc))
+         scl).
+
+  Definition call_runtime (f: string) (args: list expr) : expr:= (* TODO: review *)
+    expr_call (expr_identifier f) args.
+
+End JavaScriptAstUtil.
+
